src/RcCorrectness/Compiler.lean
@@ -1,52 +1,54 @@
-import type_system
+import Mathlib.Data.Finset.Sort
+import RcCorrectness.TypeSystem
 
-namespace rc_correctness
+namespace RcCorrectness
 
-open rc_correctness.expr
-open rc_correctness.fn_body
-open rc_correctness.lin_type
+open Expr FnBody LinType
 
-def inc_𝕆_var (x : var) (V : finset var) (F : fn_body) (βₗ : var → lin_type) : fn_body :=
-if βₗ x = 𝕆 ∧ x ∉ V then F else inc x; F
+def inc_𝕆_var (x : Var) (V : Finset Var) (F : FnBody) (βₗ : Var → LinType) : FnBody :=
+  if βₗ x = 𝕆 ∧ x ∉ V then F else incᶠᵇ x;ᶠᵇ F
 
-def dec_𝕆_var (x : var) (F : fn_body) (βₗ : var → lin_type) : fn_body :=
-if βₗ x = 𝕆 ∧ x ∉ FV F then dec x; F else F
+def dec_𝕆_var (x : Var) (F : FnBody) (βₗ : Var → LinType) : FnBody :=
+  if βₗ x = 𝕆 ∧ x ∉ fv_of_fn_body F then decᶠᵇ x;ᶠᵇ F else F
 
-def dec_𝕆 (xs : list var) (F : fn_body) (βₗ : var → lin_type) : fn_body :=
-xs.foldr (λ x acc, dec_𝕆_var x acc βₗ) F
+def dec_𝕆 (xs : List Var) (F : FnBody) (βₗ : Var → LinType) : FnBody :=
+  xs.foldr (fun x acc => dec_𝕆_var x acc βₗ) F
 
-def dec_𝕆' (xs : list var) (F : fn_body) (βₗ : var → lin_type) : fn_body :=
-xs.foldr (λ x acc, if βₗ x = 𝕆 ∧ x ∉ FV F then dec x; acc else acc) F
+def dec_𝕆' (xs : List Var) (F : FnBody) (βₗ : Var → LinType) : FnBody :=
+  xs.foldr (fun x acc => if βₗ x = 𝕆 ∧ x ∉ fv_of_fn_body F then decᶠᵇ x;ᶠᵇ acc else acc) F
 
-def C_app : list (var × lin_type) → fn_body → (var → lin_type) → fn_body
-| [] (z ≔ e; F) βₗ := z ≔ e; F
-| ((y, t)::xs) (z ≔ e; F) βₗ :=
+def C_app : List (Var × LinType) → FnBody → (Var → LinType) → FnBody
+| [], (z ≔ᶠᵇ e;ᶠᵇ F), _βₗ => z ≔ᶠᵇ e;ᶠᵇ F
+| ((y, t)::xs), (z ≔ᶠᵇ e;ᶠᵇ F), βₗ =>
   if t = 𝕆 then
-    inc_𝕆_var y ((xs.map prod.fst).to_finset ∪ FV F) (C_app xs (z ≔ e; F) βₗ) βₗ
+    inc_𝕆_var y ((xs.map Prod.fst).toFinset ∪ fv_of_fn_body F) (C_app xs (z ≔ᶠᵇ e;ᶠᵇ F) βₗ) βₗ
   else
-    C_app xs (z ≔ e; dec_𝕆_var y F βₗ) βₗ
-| xs F βₗ := F
+    C_app xs (z ≔ᶠᵇ e;ᶠᵇ dec_𝕆_var y F βₗ) βₗ
+| _xs, F, _βₗ => F
 
-def C (β : const → var → lin_type) : fn_body → (var → lin_type) → fn_body
-| (ret x) βₗ := inc_𝕆_var x finset.empty (ret x) βₗ
-| (case x of Fs) βₗ :=
-  case x of Fs.map_wf (λ F h, dec_𝕆 ((FV (case x of Fs)).sort var_le) (C F βₗ) βₗ)
-| (y ≔ x[i]; F) βₗ :=
+def C (β : Const → Var → LinType) : FnBody → (Var → LinType) → FnBody
+| (FnBody.ret x), βₗ => inc_𝕆_var x ∅ (FnBody.ret x) βₗ
+| fb@(caseᶠᵇ x ofᶠᵇ Fs), βₗ =>
+  let fvars_of_case_of_fn_body : Finset Var := fv_of_fn_body fb
+  let fvars_of_case_of_fn_body_sorted : List Var := fvars_of_case_of_fn_body.sort (· ≤ · : Var → Var → Prop)
+  caseᶠᵇ x ofᶠᵇ (Fs.map (fun F => dec_𝕆 fvars_of_case_of_fn_body_sorted (C β F βₗ) βₗ))
+| (y ≔ᶠᵇ x[ᵉi];ᶠᵇ F), βₗ =>
   if βₗ x = 𝕆 then
-    y ≔ x[i]; inc y; dec_𝕆_var x (C F (βₗ[y ↦ 𝕆])) βₗ
+    y ≔ᶠᵇ x[ᵉi];ᶠᵇ incᶠᵇ y;ᶠᵇ dec_𝕆_var x (C β F (Function.update βₗ y 𝕆)) βₗ
   else
-    y ≔ x[i]; C F (βₗ[y ↦ 𝔹])
-| (z ≔ c⟦ys…⟧; F) βₗ :=
-  C_app (ys.map (λ y, ⟨y, β c y⟩)) (z ≔ c⟦ys…⟧; C F (βₗ[z ↦ 𝕆])) βₗ
-| (z ≔ c⟦ys…, _⟧; F) βₗ :=
-  C_app (ys.map (λ y, ⟨y, β c y⟩)) (z ≔ c⟦ys…, _⟧; C F (βₗ[z ↦ 𝕆])) βₗ
-| (z ≔ x⟦y⟧; F) βₗ :=
-  C_app ([⟨x, 𝕆⟩, ⟨y, 𝕆⟩]) (z ≔ x⟦y⟧; C F (βₗ[z ↦ 𝕆])) βₗ
-| (z ≔ ⟪ys⟫i; F) βₗ :=
-  C_app (ys.map (λ y, ⟨y, 𝕆⟩)) (z ≔ ⟪ys⟫i; C F (βₗ[z ↦ 𝕆])) βₗ
-| F βₗ := F
+    y ≔ᶠᵇ x[ᵉi];ᶠᵇ C β F (Function.update βₗ y 𝔹)
+| (z ≔ᶠᵇ c⟦ys…⟧;ᶠᵇ F), βₗ =>
+  C_app (ys.map (fun y => (y, β c y))) (z ≔ᶠᵇ c⟦ys…⟧;ᶠᵇ C β F (Function.update βₗ z 𝕆)) βₗ
+| (z ≔ᶠᵇ c⟦ys…, _⟧;ᶠᵇ F), βₗ =>
+  C_app (ys.map (fun y => (y, β c y))) (z ≔ᶠᵇ c⟦ys…, _⟧;ᶠᵇ C β F (Function.update βₗ z 𝕆)) βₗ
+| (z ≔ᶠᵇ x⟦y⟧;ᶠᵇ F), βₗ =>
+  C_app [(x, 𝕆), (y, 𝕆)] (z ≔ᶠᵇ x⟦y⟧;ᶠᵇ C β F (Function.update βₗ z 𝕆)) βₗ
+| (z ≔ᶠᵇ ⟪ys⟫i;ᶠᵇ F), βₗ =>
+  C_app (ys.map (fun y => (y, 𝕆))) (z ≔ᶠᵇ ⟪ys⟫i;ᶠᵇ C β F (Function.update βₗ z 𝕆)) βₗ
+| F, _βₗ => F
 
-def C_prog (β : const → var → lin_type) (δ : program) (c : const) : fn :=
-  let (βₗ, f) := (β c, δ c) in ⟨f.ys, dec_𝕆 f.ys (C β f.F βₗ) βₗ⟩
+def C_prog (β : Const → Var → LinType) (δ : Program) (c : Const) : Fn :=
+  let (βₗ, f) := (β c, δ c)
+  ⟨f.ys, dec_𝕆 f.ys (C β f.fn_body βₗ) βₗ⟩
 
-end rc_correctness
+end RcCorrectness
