src/RcCorrectness/WellFormedness.lean
@@ -1,58 +1,75 @@
-import type_system
-import data.multiset
+import RcCorrectness.TypeSystem
 
-namespace rc_correctness
+namespace RcCorrectness
 
-open rc_correctness.expr
-open rc_correctness.fn_body
-open rc_correctness.lin_type
+section
 
-inductive fn_body_wf (β : const → var → lin_type) (δ : program) : finset var → fn_body → Prop
-notation Γ ` ⊢ `:1 F := fn_body_wf Γ F
-| ret {Γ : finset var} {x : var}
+set_option quotPrecheck false in
+set_option hygiene false in
+local notation:50 Γ " ⊢ʷᶠᵇ " fn_body => FnBodyWf β δ Γ fn_body
+
+open FnBody Expr LinType in
+inductive FnBodyWf (β : Const → Var → LinType) (δ : Program) : Finset Var → FnBody → Prop
+| ret {Γ : Finset Var} {x : Var}
   (x_def : x ∈ Γ) :
-  Γ ⊢ ret x
-| let_const_app_full {Γ : finset var} {z : var} {c : const} {ys : list var} {F : fn_body}
-  (ys_def : ys.to_finset ⊆ Γ) (arity_eq : ys.length = (δ c).ys.length)
-  (z_used : z ∈ FV F) (z_undef : z ∉ Γ) (F_wf : insert z Γ ⊢ F) :
-  Γ ⊢ (z ≔ c⟦ys…⟧; F)
-| let_const_app_part {Γ : finset var} {z : var} {c : const} {ys : list var} {F : fn_body}
-  (ys_def : ys.to_finset ⊆ Γ)
-  (no_𝔹_var : ∀ x : var, β c x ≠ 𝔹)
-  (z_used : z ∈ FV F) (z_undef : z ∉ Γ) (F_wf : insert z Γ ⊢ F) :
-  Γ ⊢ (z ≔ c⟦ys…, _⟧; F)
-| let_var_app {Γ : finset var} {z : var} {x y : var} {F : fn_body}
+  Γ ⊢ʷᶠᵇ ret x
+| let_const_app_full {Γ : Finset Var} {z : Var} {c : Const} {ys : List Var} {fn_body : FnBody}
+  (ys_def : ys.toFinset ⊆ Γ) (arity_eq : ys.length = (δ c).ys.length)
+  (z_used : z ∈ fv_of_fn_body fn_body) (z_undef : z ∉ Γ) (F_wf : insert z Γ ⊢ʷᶠᵇ fn_body) :
+  Γ ⊢ʷᶠᵇ (z ≔ᶠᵇ c⟦ys…⟧;ᶠᵇ fn_body)
+| let_const_app_part {Γ : Finset Var} {z : Var} {c : Const} {ys : List Var} {fn_body : FnBody}
+  (ys_def : ys.toFinset ⊆ Γ)
+  (no_𝔹_var : ∀ x : Var, β c x ≠ 𝔹)
+  (z_used : z ∈ fv_of_fn_body fn_body) (z_undef : z ∉ Γ) (F_wf : insert z Γ ⊢ʷᶠᵇ fn_body) :
+  Γ ⊢ʷᶠᵇ (z ≔ᶠᵇ c⟦ys…, _⟧;ᶠᵇ fn_body)
+| let_var_app {Γ : Finset Var} {z : Var} {x y : Var} {fn_body : FnBody}
   (x_def : x ∈ Γ) (y_in_Γ : y ∈ Γ)
-  (z_used : z ∈ FV F) (z_undef : z ∉ Γ) (F_wf : insert z Γ ⊢ F) :
-  Γ ⊢ (z ≔ x⟦y⟧; F)
-| let_ctor {Γ : finset var} {z : var} (i : cnstr) {ys : list var} {F : fn_body}
-  (ys_def : ys.to_finset ⊆ Γ)
-  (z_used : z ∈ FV F) (z_undef : z ∉ Γ) (F_wf : insert z Γ ⊢ F) :
-  Γ ⊢ (z ≔ ⟪ys⟫i; F)
-| let_proj {Γ : finset var} {z : var} {x : var} (i : cnstr) {F : fn_body}
+  (z_used : z ∈ fv_of_fn_body fn_body) (z_undef : z ∉ Γ) (F_wf : insert z Γ ⊢ʷᶠᵇ fn_body) :
+  Γ ⊢ʷᶠᵇ (z ≔ᶠᵇ x⟦y⟧;ᶠᵇ fn_body)
+| let_ctor {Γ : Finset Var} {z : Var} (i : Cnstr) {ys : List Var} {fn_body : FnBody}
+  (ys_def : ys.toFinset ⊆ Γ)
+  (z_used : z ∈ fv_of_fn_body fn_body) (z_undef : z ∉ Γ) (F_wf : insert z Γ ⊢ʷᶠᵇ fn_body) :
+  Γ ⊢ʷᶠᵇ (z ≔ᶠᵇ ⟪ys⟫i;ᶠᵇ fn_body)
+| let_proj {Γ : Finset Var} {z : Var} {x : Var} (i : Cnstr) {fn_body : FnBody}
   (x_def : x ∈ Γ)
-  (z_used : z ∈ FV F) (z_undef : z ∉ Γ) (F_wf : insert z Γ ⊢ F) :
-  Γ ⊢ (z ≔ x[i]; F)
-| «case» {Γ : finset var} {x : var} {Fs : list fn_body}
-  (x_def : x ∈ Γ) (Fs_wf : ∀ F ∈ Fs, Γ ⊢ F) :
-  Γ ⊢ (case x of Fs)
+  (z_used : z ∈ fv_of_fn_body fn_body) (z_undef : z ∉ Γ) (F_wf : insert z Γ ⊢ʷᶠᵇ fn_body) :
+  Γ ⊢ʷᶠᵇ (z ≔ᶠᵇ x[ᵉi];ᶠᵇ fn_body)
+| case {Γ : Finset Var} {x : Var} {Fs : List FnBody}
+  (x_def : x ∈ Γ) (Fs_wf : ∀ fn_body ∈ Fs, Γ ⊢ʷᶠᵇ fn_body) :
+  Γ ⊢ʷᶠᵇ (caseᶠᵇ x ofᶠᵇ Fs)
+end section
 
-notation β `; ` δ `; ` Γ ` ⊢ `:1 F := fn_body_wf β δ Γ F
+-- 1023 is max - 1, without it the first ;ʷᶠᵇ will fight with second ;ʷᶠᵇ
+notation β " ;ʷᶠᵇ " δ:1023 " ;ʷᶠᵇ " Γ " ⊢ʷᶠᵇ " fn_body => FnBodyWf β δ Γ fn_body
 
-inductive const_wf (β : const → var → lin_type) (δ : program) : const → Prop
-notation `⊢ `:1 c := const_wf c
-| const {c : const}
-  (F_wf : β; δ; (δ c).ys.to_finset ⊢ (δ c).F) (nd_ys : multiset.nodup (δ c).ys) :
-  ⊢ c
+section
 
-notation β `; ` δ ` ⊢ `:1 c := const_wf β δ c
+set_option quotPrecheck false in
+set_option hygiene false in
+local notation " ⊢ʷᶜ " c => ConstWf β δ c
 
-inductive program_wf (β : const → var → lin_type) : program → Prop
-notation `⊢ `:1 δ := program_wf δ
-| program {δ : program}
-  (const_wf : ∀ c : const, β; δ ⊢ c) :
-  ⊢ δ
+open FnBody Expr LinType in
+inductive ConstWf (β : Const → Var → LinType) (δ : Program) : Const → Prop
+| const {c : Const}
+  (F_wf : β;ʷᶠᵇ δ;ʷᶠᵇ (δ c).ys.toFinset ⊢ʷᶠᵇ (δ c).fn_body) (nd_ys : (δ c).ys.Nodup) :
+  ⊢ʷᶜ c
+end section
 
-notation β ` ⊢ `:1 δ := program_wf β δ
+notation β " ;ʷᶜ " δ " ⊢ʷᶜ " c => ConstWf β δ c
 
-end rc_correctness
+section
+
+set_option quotPrecheck false in
+set_option hygiene false in
+local notation " ⊢ᵖʷ " δ => ProgramWf β δ
+
+open FnBody Expr LinType in
+inductive ProgramWf (β : Const → Var → LinType) : Program → Prop
+| program {δ : Program}
+  (const_wf : ∀ c : Const, β ;ʷᶜ δ ⊢ʷᶜ c) :
+  ⊢ᵖʷ δ
+end section
+
+notation β " ⊢ᵖʷ " δ => ProgramWf β δ
+
+end
