src/RcCorrectness.lean
@@ -1,6 +1,6 @@
-import RcCorrectness.Util
 import RcCorrectness.Ast
 import RcCorrectness.TypeSystem
-import RcCorrectness.Compiler
 import RcCorrectness.WellFormedness
+import RcCorrectness.Compiler
 import RcCorrectness.Theorem
+-- import RcCorrectness.Util
